\documentclass[letterpaper,11pt]{article}

\usepackage{amsmath}
\usepackage{amssymb}
\usepackage{bm}
\usepackage[hmargin=1.25in,vmargin=1in]{geometry}
\usepackage{booktabs}
\usepackage{graphicx}
\usepackage{hyperref}
\usepackage{lmodern}
\usepackage{microtype}
\usepackage{pdflscape}
\usepackage{subcaption}

\title{Coursework 8: STAT 570}
\author{Philip Pham}
\date{\today}

\begin{document}
\maketitle
\begin{enumerate}
\item Consider n experiments with $Z_{ij}$ , $j = 1,2,\ldots, N_i$, the binary
  outcomes within cluster (experiment) $i$ with $Y_i = \sum^N_{j=1} Z_{ij}$,
  $i = 1,\ldots,n$.
  \begin{enumerate}
  \item By writing
    \begin{equation}
      \operatorname{var}\left(Y_i\right)
      = \sum_{j=1}^{N_i} \operatorname{var}\left(Z_{ij}\right)
      + \sum_{j=1}^{N_i}\sum_{j \neq k} \operatorname{cov}\left(Z_{ij}, Z_{ik}\right),
      \label{eqn:p1_var_yi}
    \end{equation}
    show that
    \begin{equation}
      \operatorname{var}\left(Y_i\right)
      = N_ip_i\left(1 - p_i\right) \times
      \left[1 + \left(N_i - 1\right)\tau_i^2\right],
      \label{eqn:p1_var_yi_result}
    \end{equation}
    where $p_i = \mathbb{E}\left[Z_{ij}\right]$ and $\tau_i^2$ is the
    correlation of outcomes within cluster $i$.

    \begin{description}
    \item[Solution:] Using the variance for a Bernoulli random variable and the
      definition of the correlation coefficient, we have that
      \begin{align}
        \operatorname{var}\left(Z_{ij}\right)
        &= p_i\left(1 - p_i\right) \label{eqn:p1_var_cov}\\
        \operatorname{cov}\left(Z_{ij}, Z_{ik}\right)
        &= \tau_i^2p_i\left(1 - p_i\right)~\text{for}~j \neq k.
          \nonumber
      \end{align}
      
      Since $Z_{ij}$ are identically distributed for different $j$, we can
      rewrite Equation \ref{eqn:p1_var_yi} as
      \begin{equation}
        \operatorname{var}\left(Y_i\right)
        = N_i\operatorname{var}\left(Z_{i1}\right) +
        N_i\left(N_i - 1\right)\operatorname{cov}\left(Z_{i1},Z_{i2}\right).
        \label{eqn:p1_var_yi_simplified} 
      \end{equation}

      Applying Equation \ref{eqn:p1_var_cov} to Equation
      \ref{eqn:p1_var_yi_simplified}, we have the result
      \begin{align*}
        \operatorname{var}\left(Y_i\right)
        &= N_ip_i\left(1-p_i\right)
          + N_i\left(N_i - 1\right) \tau_i^2p_i\left(1-p_i\right) \\
        &= N_ip_i\left(1-p_i\right) \times \left[
          1 + \left(N_i - 1\right) \tau_i^2
          \right]
      \end{align*}
      as desired.
    \end{description}
  \item Consider the model
    \begin{align}
      Y_i \mid q_i &\sim \operatorname{Binomial}\left(N_i,q_i\right) \\
      q_i &\sim \operatorname{Beta}\left(a_i,b_i\right),
            \label{eqn:p1_model}
    \end{align}
    where we can parameterize as $a_i = dp_i$, $b_i = d\left(1-p_i\right)$, so
    that
    \begin{align}
      \mathbb{E}\left[q_i\right]
      &= p_i = \frac{a_i}{d} \\
      \operatorname{var}\left(q_i\right)
      &= \frac{p_1\left(1 - p_i\right)}{d+1}.
    \end{align}
    Obtain the marginal moments and show that the variance is of the form in
    Equation \ref{eqn:p1_var_yi_result}, and identify $\tau_i^2$.

    \begin{description}
    \item[Solution:] We have that
      \begin{align}
        \mathbb{P}\left(Y_i = y\right)
        &= \int_0^1 \mathbb{P}\left(Y_i \mid q_i\right)p\left(q_i\right)
          \,\mathrm{d}q_i \nonumber\\
        &= \int_0^1 \left(
          {N_i \choose y }q_i^y \left(1 - q_i\right)^{N_i - y}
          \right)
          \left(
          \frac{\Gamma\left(a_i + b_i\right)}
          {\Gamma\left(a_i\right)\Gamma\left(b_i\right)}
          q_i^{a_i - 1}\left(1 - q_i\right)^{b_i - 1}
          \right)
          \,\mathrm{d}q_i \nonumber\\
        &= {N_i \choose y}
          \frac{\Gamma\left(a_i + b_i\right)}
          {\Gamma\left(a_i\right)\Gamma\left(b_i\right)}
          \int_0^1 
          q_i^{a_i + y - 1} \left(1 - q_i\right)^{b_i + N_i - y - 1}
          \,\mathrm{d}q_i \nonumber\\
        &= {N_i \choose y}
          \left(
          \frac{\Gamma\left(a_i + b_i\right)}
          {\Gamma\left(a_i\right)\Gamma\left(b_i\right)}
          \right)
          \left(
          \frac{\Gamma\left(y + a_i\right)\Gamma\left(
          N_i - y + b_i
          \right)}
          {\Gamma\left(N_i + a_i + b_i\right)}
          \right),
          \label{eqn:p1_beta_binomial}
      \end{align}
      so $Y_i \sim \operatorname{BetaBinomial}\left(
        N_i, a_i, b_i\right)$.

      Using Equation \ref{eqn:p1_beta_binomial}, the expectation of $Y_i$ is
      \begin{equation}
        \mathbb{E}\left[Y_i\right]
        = \sum_{y=0}^{N_i}y\mathbb{P}\left(
        Y_i = y
          \right)
          = \sum_{y=1}^{N_i}y\mathbb{P}\left(
          Y_i = y
        \right).
        \label{eqn:p1_expectation_definition}
      \end{equation}

      Note that when $N_i = 1$, Equation \ref{eqn:p1_expectation_definition}
      trivially becomes $a_i/\left(a_i + b_i\right)$. In general, we can show
      that $\displaystyle\mathbb{E}\left[Y_i\right] = N_i\frac{a_i}{a_i +
        b_i}$. With the $N_i = 1$ base case established, we now have
      % \tiny{
        \begin{align}
          \mathbb{E}\left[Y_i\right]
        &= \sum_{y=1}^{N_i}y\mathbb{P}\left(Y_i = y\right) \nonumber\\
        &= \sum_{y=1}^{N_i} y {N_i \choose y}
          \left(
          \frac{\Gamma\left(a_i + b_i\right)}
          {\Gamma\left(a_i\right)\Gamma\left(b_i\right)}
          \right)
          \left(
          \frac{\Gamma\left(y + a_i\right)\Gamma\left(
          N_i - y + b_i
          \right)}
          {\Gamma\left(N_i + a_i + b_i\right)}
          \right) \nonumber\\
          &= \frac{N_i}{N_i - 1 + a_i + b_i} \sum_{y=1}^{N_i}
            \left(y - 1 + a_i\right)
            \operatorname{BetaBinomial}_{N_i - 1,a_i,b_i}
            \left(y - 1\right) \nonumber\\
        &= \frac{N_i}{N_i - 1 + a_i + b_i}
          \left(
          \frac{\left(N_i - 1\right)a_i}{a_i + b_i} + a_i
          \right) = N_i\frac{a_i}{a_i + b_i}
          \label{eqn:p1_expectation_derivation}
        \end{align}
      % }
      \normalsize
      as expected. Substituting, we have that
      \begin{equation}
        \mathbb{E}\left[
          Y_i \right]
        = N_i\frac{dp_i}{dp_i + d\left(1 - p_i\right)}  = N_ip_i.
        \label{eqn:p1_expectation_substitution}
      \end{equation}
      
      Using a similar strategy as in Equation
      \ref{eqn:p1_expectation_derivation}, we have that
      \begin{equation}
        \mathbb{E}\left[Y_i\left(Y_i - 1\right)\right]
        = 
        = \mathbb{E}\left[Y_i^2\right] - \mathbb{E}\left[Y_i\right].
      \end{equation}
          
    \end{description}
\end{enumerate}
\end{enumerate}
\end{document}
